

%-------------------------------------------------------------------------------
% Dokumenten Klasse
\documentclass[
	final,
	a4paper,
	oneside,
	parskip=full,
	headings=standardclasses,
	headings=big,
	pointednumbers,
    fleqn
]{scrartcl}

%-------------------------------------------------------------------------------
% Packete nutzen
\usepackage{ngerman,palatino,setspace}
\usepackage[T1]{fontenc}
\usepackage[utf8]{inputenc}
\usepackage[left=20mm,right=20mm,top=10mm,bottom=25mm]{geometry}
\usepackage{amsmath}
\usepackage{amssymb}
\usepackage{mathtools}

%-------------------------------------------------------------------------------
% FÃ¼r enumerate
\usepackage{enumitem}
\setlist[enumerate]{
    wide=0pt,
    leftmargin=*,
    itemsep=-1ex,
    parsep=2ex,
    labelsep=1ex,
    label=\alph*)
}


%-------------------------------------------------------------------------------
% 
\usepackage{xparse}
% 1: Subscription  (default: '')
% 2: Funktion Name (default: 'f')
% 3: Argument      (default: 'x')
% \fx         = f(x)
% \fx[1]      = f_1(x)
% \fx[][u]    = u(x)
% \fx[][u][x] = u(x)
% \fx[][f][u] = f(u)
\NewDocumentCommand{\fx}{ O{} O{f} O{x} }{{#2_{#1}{\left( #3 \right)}}}
\NewDocumentCommand{\dfx}{ O{} O{f} O{x} }{{#2'_{#1}{\left( #3 \right)}}}
\newcommand{\e}{\mathrm{e}}
\newcommand{\kl}[1]{{\left( #1 \right)}}

%-------------------------------------------------------------------------------
% Dokument
\begin{document}

    \subsection*{Ableitungsregeln}
    
    \renewcommand{\arraystretch}{1.25}
    \begin{tabular}{lll}
        Faktorregel  & $ y = C \cdot \fx$                   & $ y' = C \cdot \dfx $ \\
                     & $ y = 5 \cdot x^2 $                  & $ y' = 5 \cdot 2 \cdot x$ \\
        Summenregel  & $ y = \fx[1] + \ldots +  \fx[n] $    & $ y' = \dfx[1] + \ldots + \dfx[n] $\\
                     & $ y = x^2 + x^3$                     & $ y' = 2 \cdot x + 3 \cdot x^2$ \\
        Produktregel & $ y = \fx[][u] \cdot \fx[][v] $      & $ y' = \fx[][u] \cdot \dfx[][v] + \dfx[][u] \cdot \fx[][v] $ \\
                     & $ y = x^2 \cdot e^{2x}  $            & $ y' = x^2 \cdot 2\cdot e^{2x} + 2\cdot x \cdot e^{2x} $ \\
                     &                                      & $ y' = {\left( 2x^2 + 2x \right)} e^{2x} $ \\
        Kettenregel  & $ y = f\kl{u\kl{x}} $                & $ y' = \dfx[][f][u] \cdot \dfx[][u][x] $ \\
                     & $ y = f\kl{x^2 - 5}, \; f = x^2 $    & $ y' = 2 u \cdot 2x = 4x \kl{x^2 - 5} $ \\
                     & $ y = \ln\kl{1 + x^2} $              & $ y' = \frac{1}{u} \cdot 2x = \frac{2x}{1 + x^2} $ \\
    \end{tabular} \\
\end{document}
